theories/Pre_orders/Must/Alternative_Preorder/Acceptance_Set/Soundness.v
@@ -580,8 +580,8 @@ Definition bhv_pre_cond1__x `{FiniteImagegLts P A, FiniteImagegLts Q A} (ps : gs
 Notation "ps ≼ₓ1 q" := (bhv_pre_cond1__x ps q) (at level 70).
 
 Definition bhv_pre_cond2__x `{
-  @FiniteImagegLts P A H gLtsP, PreAP : @PreExtAction A H P PreA PreA_eq PreA_countable 𝝳 gLtsP,
-  @FiniteImagegLts Q A H gLtsQ, PreAQ : @PreExtAction A H Q PreA PreA_eq PreA_countable 𝝳 gLtsQ}
+  @FiniteImagegLts P A H gLtsP, PreAP : @PreExtAction A H P FinA PreA PreA_eq PreA_countable 𝝳  Φ gLtsP,
+  @FiniteImagegLts Q A H gLtsQ, PreAQ : @PreExtAction A H Q FinA PreA PreA_eq PreA_countable 𝝳  Φ gLtsQ}
   (ps : gset P) (q : Q) :=
   forall s q',
     q ⟹[s] q' -> q' ↛ ->
@@ -595,8 +595,8 @@ Notation "ps ≼ₓ2 q" := (bhv_pre_cond2__x ps q) (at level 70).
 Notation "ps ≼ₓ q" := (bhv_pre_cond1__x ps q /\ bhv_pre_cond2__x ps q) (at level 70).
 
 Lemma alt_set_singleton_iff `{
-  @FiniteImagegLts P A H gLtsP, PreAP : @PreExtAction A H P PreA PreA_eq PreA_countable 𝝳 gLtsP,
-  @FiniteImagegLts Q A H gLtsQ, PreAQ : @PreExtAction A H Q PreA PreA_eq PreA_countable 𝝳 gLtsQ}
+  @FiniteImagegLts P A H gLtsP, PreAP : @PreExtAction A H P FinA PreA PreA_eq PreA_countable 𝝳 Φ gLtsP,
+  @FiniteImagegLts Q A H gLtsQ, PreAQ : @PreExtAction A H Q FinA PreA PreA_eq PreA_countable 𝝳 Φ gLtsQ}
   (p : P) (q : Q) : p ≼ q <-> {[ p ]} ≼ₓ q.
 Proof.
   split.
@@ -616,8 +616,8 @@ Lemma bhvleqone_preserved_by_tau `{
 Proof. intros halt1 l s mem. eapply cnv_preserved_by_lts_tau; eauto. Qed.
 
 Lemma bhvx_preserved_by_tau `{
-  @FiniteImagegLts P A H gLtsP, PreAP : @PreExtAction A H P PreA PreA_eq PreA_countable 𝝳 gLtsP,
-  @FiniteImagegLts Q A H gLtsQ, PreAQ : @PreExtAction A H Q PreA PreA_eq PreA_countable 𝝳 gLtsQ}
+  @FiniteImagegLts P A H gLtsP, PreAP : @PreExtAction A H P FinA PreA PreA_eq PreA_countable 𝝳 Φ gLtsP,
+  @FiniteImagegLts Q A H gLtsQ, PreAQ : @PreExtAction A H Q FinA PreA PreA_eq PreA_countable 𝝳 Φ gLtsQ}
   (ps : gset P) (q q' : Q) : q ⟶ q' -> ps ≼ₓ q -> ps ≼ₓ q'.
 Proof.
   intros l (halt1 & halt2).
@@ -643,8 +643,8 @@ Proof.
 Qed.
 
 Lemma bhvx_preserved_by_mu `{
-  @FiniteImagegLts P A H gLtsP, PreAP : @PreExtAction A H P PreA PreA_eq PreA_countable 𝝳 gLtsP,
-  @FiniteImagegLts Q A H gLtsQ, PreAQ : @PreExtAction A H Q PreA PreA_eq PreA_countable 𝝳 gLtsQ}
+  @FiniteImagegLts P A H gLtsP, PreAP : @PreExtAction A H P FinA PreA PreA_eq PreA_countable 𝝳 Φ gLtsP,
+  @FiniteImagegLts Q A H gLtsQ, PreAQ : @PreExtAction A H Q FinA PreA PreA_eq PreA_countable 𝝳 Φ gLtsQ}
   (ps0 : gset P) (q : Q) μ ps1 q' (htp : forall p, p ∈ ps0 -> terminate p) :
   q ⟶[μ] q' 
     -> wt_set_from_pset_spec ps0 [μ] ps1 
@@ -674,8 +674,8 @@ Proof.
 Qed.
 
 Lemma bhvx_mu_ex `{
-  @FiniteImagegLts P A H gLtsP, PreAP : @PreExtAction A H P PreA PreA_eq PreA_countable 𝝳 gLtsP,
-  @FiniteImagegLts Q A H gLtsQ, PreAQ : @PreExtAction A H Q PreA PreA_eq PreA_countable 𝝳 gLtsQ}
+  @FiniteImagegLts P A H gLtsP, PreAP : @PreExtAction A H P FinA PreA PreA_eq PreA_countable 𝝳 Φ gLtsP,
+  @FiniteImagegLts Q A H gLtsQ, PreAQ : @PreExtAction A H Q FinA PreA PreA_eq PreA_countable 𝝳 Φ gLtsQ}
   (ps : gset P) (q q' : Q) μ
   : ps ≼ₓ q -> (forall p, p ∈ ps -> p ⇓ [μ]) ->
     q ⟶[μ] q' -> exists p', wt_set_from_pset_spec1 ps [μ] {[ p' ]}.
@@ -692,10 +692,12 @@ Qed.
 
 Lemma ungood_must_st_nleqx `{
   @gLtsObaFW P A H gLtsP gLtsEqP gLtsObaP, !FiniteImagegLts P A,
-  PreAP : @PreExtAction A H P PreA PreA_eq PreA_countable 𝝳 gLtsP,
+  PreAP : @PreExtAction A H P FinA PreA PreA_eq PreA_countable 𝝳 Φ gLtsP,
   @gLtsObaFW Q A H gLtsQ gLtsEqQ gLtsObaQ, !FiniteImagegLts Q A,
-  PreAQ : @PreExtAction A H Q PreA PreA_eq PreA_countable 𝝳 gLtsQ,
+  PreAQ : @PreExtAction A H Q FinA PreA PreA_eq PreA_countable 𝝳 Φ gLtsQ,
   gLtsE : !gLts E A, !gLtsEq E A, !Good E A good}
+
+  `{AbE : @AbsAction A H E FinA gLtsE Φ}
 
   `{@Prop_of_Inter P E A parallel_inter H gLtsP gLtsE}
   `{@Prop_of_Inter Q E A parallel_inter H gLtsQ gLtsE}
@@ -736,21 +738,32 @@ Proof.
       eapply Hyp in nb as (tr1 & tr2); eauto.
       eapply (lts_refuses_spec2 (q ▷ e)); eauto. exists (q'', e'').
       eapply ParSync; eauto.
-    + assert (𝝳 μ2 ∈ pre_co_actions_of p') as mem'. 
-      { eapply preactions_of_spec. exists μ1. repeat split; eauto.
+    + assert (μ2 ∈ co_actions_of p') as some_co_action_of_p.
+      { exists μ1. repeat split; eauto.
         eapply lts_refuses_spec2;eauto. symmetry in eq; eauto. }
-      eapply sub in mem'. eapply preactions_of_spec in mem'.
-      destruct mem' as (μ'1 & Tr & duo & b). 
-      eapply lts_refuses_spec1 in Tr as (q'' & tr'').
-      eapply (lts_refuses_spec2 (q,e)). exists (q'', e'').
+      eapply preactions_of_fin_test_spec1 in some_co_action_of_p.
+      eapply preactions_of_spec in some_co_action_of_p.
+      eapply sub in some_co_action_of_p.
+      eapply preactions_of_spec in some_co_action_of_p.
+      eapply preactions_of_fin_test_spec2 in some_co_action_of_p as (μ' & mem' & eq').
+      assert (¬ e ↛[μ']) as Tr_Test.
+      { eapply abstraction_test_spec. exact eq'. apply lts_refuses_spec2. eauto. }
+      destruct mem' as (μ'1 & Tr & duo & b).
+      eapply lts_refuses_spec1 in Tr_Test as (e' & Tr').
+      eapply lts_refuses_spec1 in Tr as (q' & Tr).
+      eapply (lts_refuses_spec2 (q,e)). exists (q', e').
       symmetry in duo.
       eapply ParSync; eauto. eauto.
 Qed.
 
 Lemma stability_nbhvleqtwo `{
-  @gLtsObaFW P A H gLtsP gLtsEqP gLtsObaP, !FiniteImagegLts P A, PreAP : @PreExtAction A H P PreA PreA_eq PreA_countable 𝝳 gLtsP,
-  @gLtsObaFW Q A H gLtsQ gLtsEqQ gLtsObaQ, !FiniteImagegLts Q A, PreAQ : @PreExtAction A H Q PreA PreA_eq PreA_countable 𝝳 gLtsQ,
+  @gLtsObaFW P A H gLtsP gLtsEqP gLtsObaP, !FiniteImagegLts P A,
+  PreAP : @PreExtAction A H P FinA PreA PreA_eq PreA_countable 𝝳 Φ gLtsP,
+  @gLtsObaFW Q A H gLtsQ gLtsEqQ gLtsObaQ, !FiniteImagegLts Q A,
+  PreAQ : @PreExtAction A H Q FinA PreA PreA_eq PreA_countable 𝝳 Φ gLtsQ,
   gLtsE : !gLts E A, !gLtsEq E A, !Good E A good}
+
+  `{AbE : @AbsAction A H E FinA gLtsE Φ}
 
   `{@Prop_of_Inter P E A parallel_inter H gLtsP gLtsE}
   `{@Prop_of_Inter Q E A parallel_inter H gLtsQ gLtsE}
@@ -769,10 +782,12 @@ Qed.
 
 Lemma soundnessx `{
   @gLtsObaFW P A H gLtsP gLtsEqP gLtsObaP, !FiniteImagegLts P A,
-  PreAP : @PreExtAction A H P PreA PreA_eq PreA_countable 𝝳 gLtsP,
+  PreAP : @PreExtAction A H P FinA PreA PreA_eq PreA_countable 𝝳 Φ gLtsP,
   @gLtsObaFW Q A H gLtsQ gLtsEqQ gLtsObaQ, !FiniteImagegLts Q A,
-  PreAQ : @PreExtAction A H Q PreA PreA_eq PreA_countable 𝝳 gLtsQ,
+  PreAQ : @PreExtAction A H Q FinA PreA PreA_eq PreA_countable 𝝳 Φ gLtsQ,
   @gLtsObaFB E A H gLtsE gLtsEqE gLtsObaE, !FiniteImagegLts E A, !Good E A good}
+
+  `{AbE : @AbsAction A H E FinA gLtsE Φ}
 
   `{@Prop_of_Inter P E A parallel_inter H gLtsP gLtsE}
   `{@Prop_of_Inter Q E A parallel_inter H gLtsQ gLtsE}
@@ -825,10 +840,12 @@ Qed.
 
 Lemma soundness_fw `{
   @gLtsObaFW P A H gLtsP gLtsEqP V, !FiniteImagegLts P A,
-  PreAP : @PreExtAction A H P PreA PreA_eq PreA_countable 𝝳 gLtsP,
+  PreAP : @PreExtAction A H P FinA PreA PreA_eq PreA_countable 𝝳 Φ gLtsP,
   @gLtsObaFW Q A H gLtsQ gLtsEqQ T, !FiniteImagegLts Q A,
-  PreAQ : @PreExtAction A H Q PreA PreA_eq PreA_countable 𝝳 gLtsQ,
+  PreAQ : @PreExtAction A H Q FinA PreA PreA_eq PreA_countable 𝝳 Φ gLtsQ,
   @gLtsObaFB E A H gLtsE gLtsEqE W, !FiniteImagegLts E A, !Good E A good }
+
+  `{AbE : @AbsAction A H E FinA gLtsE Φ}
 
   `{@Prop_of_Inter P E A parallel_inter H gLtsP gLtsE}
   `{@Prop_of_Inter Q E A parallel_inter H gLtsQ gLtsE}
@@ -845,6 +862,8 @@ Lemma soundness `{
   @gLtsObaFB Q A H gLtsQ gLtsEqQ T, !FiniteImagegLts Q A,
   @gLtsObaFB E A H gLtsE gLtsEqE W, !FiniteImagegLts E A, !Good E A good }
 
+  `{AbE : @AbsAction A H E FinA gLtsE Φ}
+
   `{@Prop_of_Inter P E A parallel_inter H gLtsP gLtsE}
   `{@Prop_of_Inter Q E A parallel_inter H gLtsQ gLtsE}
 
@@ -854,8 +873,8 @@ Lemma soundness `{
   `{@Prop_of_Inter Q (mb A) A fw_inter H gLtsQ MbgLts}
   `{@Prop_of_Inter (Q * mb A) E A parallel_inter H (inter_lts fw_inter) gLtsE}
 
-  `{PreAP : @PreExtAction A H (P * mb A) PreA PreA_eq PreA_countable 𝝳 (inter_lts fw_inter),
-    PreAQ : @PreExtAction A H (Q * mb A) PreA PreA_eq PreA_countable 𝝳 (inter_lts fw_inter)}
+  `{PreAP : @PreExtAction A H (P * mb A) FinA PreA PreA_eq PreA_countable 𝝳 Φ (inter_lts fw_inter),
+    PreAQ : @PreExtAction A H (Q * mb A) FinA PreA PreA_eq PreA_countable 𝝳 Φ (inter_lts fw_inter)}
   (p : P) (q : Q) : p ▷ ∅ ≼ q ▷ ∅ -> p ⊑ q.
 Proof.
   intros halt e hm.
